Fix order of get/set arguments

src/Hlist.v
@@ -1,6 +1,7 @@
 Require Import List.
 Import List.ListNotations.
 Open Scope list.
+
 Require Import Coq.Program.Equality.
 
 Set Implicit Arguments.
@@ -28,7 +29,7 @@ Section hlist.
   (** Adapted from CPDT DataStruct hlist.
 
       In Coq v8.5beta2 at least, the return annotations are unnecessary. *)
-  Fixpoint get types (l: hlist types) : member types -> B elm :=
+  Fixpoint get_impl types (l: hlist types) : member types -> B elm :=
     match l with
     | HNil => fun mem =>
                match mem in member ls' return (match ls' with
@@ -47,20 +48,26 @@ Section hlist.
                                                        end) with
                        | HFirst _ => fun x _ => x
                        | HNext _ mem' => fun _ get_mls' => get_mls' mem'
-                       end x (get mls')
+                       end x (get_impl mls')
     end.
 
-  Fixpoint set types (l: hlist types) (new: B elm) : member types -> (hlist types) :=
+  Fixpoint set_impl types (l: hlist types) (new: B elm) : member types -> (hlist types) :=
     match l with
     | HNil => fun mem => HNil
     | HCons x mls' => fun mem =>
                        match mem in member ls' with
                        | HFirst _ => fun x _ => HCons new mls'
                        | HNext _ mem' => fun x set_mls' => HCons x (set_mls' mem')
-                       end x (set mls' new)
+                       end x (set_impl mls' new)
     end.
 
 End hlist.
+
+Definition get {A} {B: A -> Type} {types} {elm: A}
+           (m: member elm types) (l: hlist B types) := get_impl l m.
+
+Definition set {A} {B: A -> Type} {types} {elm: A}
+           (m: member elm types) (new: B elm) (l: hlist B types) := set_impl l new m.
 
 Arguments HCons [A] [B] [a] [types] el xs.
 Arguments HNil [A] [B].
@@ -72,18 +79,19 @@ Module Examples.
   Local Example types := [nat; bool; nat].
   Local Example someValues : hlist (fun T : Set => T) types := HCons 5 (HCons true (HCons 3 HNil)).
 
-  Eval simpl in get someValues HFirst.
-  Eval simpl in get someValues (HNext HFirst).
+  Eval simpl in get HFirst someValues.
+  Eval simpl in get (HNext HFirst) someValues.
 
-  Eval simpl in set someValues false (HNext HFirst).
+  Eval simpl in set (HNext HFirst) false someValues.
 
 End Examples.
 
 Theorem get_set : forall A B (types: list A)
                     (l : hlist B types)
                     (elm:A) (m: member elm types) v,
-    get (set l v m) m = v.
+    get m (set m v l) = v.
 Proof.
+  unfold get, set.
   induction l; intros.
   inversion m.
 
@@ -95,8 +103,9 @@ Theorem get_set_other : forall A B (types: list A)
                           (elm1:A) (m1: member elm1 types)
                           (elm2:A) (m2: member elm2 types) v,
     member_index m1 <> member_index m2 ->
-    get (set l v m1) m2 = get l m2.
+    get m2 (set m1 v l) = get m2 l.
 Proof.
+  unfold get, set.
   induction l; intros.
   inversion m1.
 
@@ -116,6 +125,9 @@ Ltac simpl_get_set_hyp H :=
   repeat (rewrite get_set in H ||
                                rewrite get_set_other in H by (cbn; auto));
   auto.
+
+(* certainly we don't want users to reason about get_impl and set_impl *)
+Global Opaque get set.
 
 Tactic Notation "simpl_get_set" := simpl_get_set_goal.
 (* TODO: debug this notation not working *)
